SimModSem compiles

theories/System.v
@@ -17,13 +17,13 @@ Section SYSMODSEM.
 
   Definition globalenv: genvtype := skenv_link.
 
-  Definition skenv: SkEnv.t := admit "".
-    (* (Genv_map_defs skenv_link)(fun _ gd => *)
-    (*                              match gd with *)
-    (*                              | Gfun (External ef) => Some (Gfun (Internal (ef_sig (ef)))) *)
-    (*                              | Gfun _ => None *)
-    (*                              | Gvar gv => Some gd *)
-    (*                              end). *)
+  Definition skenv: SkEnv.t :=
+    (Genv.map_defs skenv_link)(fun gd =>
+                                 match gd with
+                                 | Gfun (External ef) => Some (Gfun (Internal (ef_sig (ef))))
+                                 | Gfun _ => None
+                                 | Gvar gv => Some gd
+                                 end).
 
   (* Lemma skenv_globlaenv_equiv: Senv.equiv skenv globalenv. *)
   (* Proof. *)
@@ -47,7 +47,7 @@ Section SYSMODSEM.
   Inductive step (se: Senv.t) (ge: genvtype): state -> trace -> state -> Prop :=
   | step_intro
       ef fptr vs m0 v m1 tr
-      (FPTR: (Genv.find_funct ge) fptr = Some (External _ ef))
+      (FPTR: (Genv.find_funct ge) fptr = Some (External ef))
       (EXTCALL: external_call ef (SkEnv.to_senv ge) vs m0 tr v m1):
       step se ge (Callstate fptr vs m0) tr (Returnstate v m1).
 
